cem_cbn_bisim.v
@@ -1,5 +1,5 @@
-Require Import bisim db List.
-Require cem cbn.
+Require Import bisim db List NaryFunctions.
+Require cem cbn expr expr_db_nat.
 
 Inductive state_rel : relation cem.configuration cbn.configuration := 
   | init : forall t e,
@@ -11,7 +11,23 @@ Inductive state_rel : relation cem.configuration cbn.configuration :=
            cbn.step b b' ->
            state_rel a' b'.
 
+Fixpoint subst_cbn_config (st : cbn.configuration) : expr.tm := match st with
+  | cbn.st vs e => match vs with
+    | nil => e
+    | (x,m)::hs => subst_cbn_config (cbn.st hs (cbn.subst x m e))
+    end
+  end.
+
+Fixpoint subst_cem_config (st : cem.configuration) : expr_db_nat.expr := match st with
+  | cem.st nil 
+  | 
+
 Theorem cem_cbn_bisim : bisim state_rel cem.step cbn.step.
 unfold bisim.
 intros. split. 
-  intros. inversion H.  
+  intros. induction H. destruct H. inversion H0. symmetry in H.
+  apply app_cons_not_nil in H. inversion H.  apply ex_intro with (cbn.st nil
+  (expr.abs v b)). assert (cbn.step (cbn.st nil (expr.abs v b)) (cbn.st nil
+  (expr.abs v b))).  apply cbn.Abs. split. assumption. 
+    apply init. with (cem.st nil (cem.close (expr_db_nat.lam b') 0))
+                    (cbn.st nil (expr.abs v b)).
