Makefile
@@ -1,4 +1,8 @@
 COQC := coqc
+sources = expr expr_db_nat bisim db cem cbn
+
+all: ${sources}
+
 %: %.v
 	${COQC} $<
 
